Avanzando un poco mas"

RAlist/test.fst
@@ -8,6 +8,8 @@ open FStar.Tactics
 (* Some util functions I couldnt find
 *)
 
+(* Power *)
+
 val pow : a:pos -> e:nat -> pos
 let rec pow a e = match e with
     | 0 -> 1
@@ -23,6 +25,33 @@ let pow_dec_on_e e1 e2 a = begin
   pow_distr_sums_on_e (e2 - e1) e1 a
 end
 
+(* List lemmas *)
+
+val lemma_append_length: l1:list 'a -> l2:list 'a
+                -> Lemma (requires True)
+                        (ensures (length ( l1 @ l2) = length l1 + length l2))
+let rec lemma_append_length l1 l2 = match l1 with
+    | [] -> ()
+    | hd::tl -> lemma_append_length tl l2
+
+// Definition of @
+//val helper_lemma : #b:eqtype -> x:b -> l1:list b -> l2:list b -> Lemma ((x::l1) @ l2 = x::(l1@l2))
+//let rec helper_lemma #b x l1 l2 = ()
+
+val lemma_append_assoc : #b:eqtype -> l1:list b -> l2:list b -> l3:list b -> Lemma ((l1@l2)@l3 = l1@(l2@l3))
+let rec lemma_append_assoc #b l1 l2 l3 = match l1 with
+  | [] -> ()
+  | hd::tl -> lemma_append_assoc tl l2 l3
+// Simple enough, shouldnt need it
+(*val random_lemma : 
+                 #b:Type -> 
+                 x:b -> 
+                 l1:list b -> 
+                 l2:list b -> 
+                 Lemma (length (x :: l1 @ l2) = 1 + length l1 + length l2)
+let rec random_lemma #b x l1 l2 = lemma_append_length l1 l2
+*)
+
 (*  comBiTree
     comBitree is a non empty COMplete BInary TREE with the height of the tree at type level
 *)
@@ -34,55 +63,50 @@ type comBiTree 'a : (x:pos) -> Type =
 val treeHeight : (#x:pos) -> comBiTree 'a x ->  y:pos{y = x}
 let rec treeHeight (t:comBiTree 'a 'n) = match t with
     | Leaf _ -> 1
-    | Branch _ t2 _ -> 1 + treeHeight t2
+    | Branch _ t1 t2 -> (
+      assert(treeHeight t1 = treeHeight t2);
+      1 + treeHeight t2
+    )
 
-val treeSize : (#x:pos) -> comBiTree 'a x ->  y:pos{y = pow2 x - 1}
+val treeSize : (#x:pos) -> comBiTree 'a x ->  y:pos{y = (pow2 x) - 1}
 let rec treeSize (t:comBiTree 'a 'n) = match t with
   | Leaf _ -> 1
   | Branch _ t1 t2 -> 1 + treeSize t1 + treeSize t2
 
-val preorder : (#x:pos) -> (#b:Type) -> t:comBiTree b x -> l:list b
+val tree_size_gives_height : #b:Type -> #h1:pos -> #h2:pos -> t1:comBiTree b h1 -> t2:comBiTree b h2 -> Lemma (requires treeSize t1 = treeSize t2) (ensures h1 = h2)
+let rec tree_size_gives_height #b #h1 #h2 t1 t2 = match t1 with
+  | Leaf _ -> begin match t2 with
+    | Leaf _ -> ()
+    | Branch _ t21 t22 -> ()
+  end
+  | Branch _ t11 t12 -> begin match t2 with
+    | Leaf _ -> ()
+    | Branch _ t21 t22 -> tree_size_gives_height t11 t21
+  end
+
+val treeRoot : #x:pos -> #b:Type -> comBiTree b x -> b
+let treeRoot #x #b t = match t with
+  | Leaf a -> a
+  | Branch a _ _ -> a
+
+val preorder : (#x:pos) -> (#b:Type) -> t:comBiTree b x -> l:list b{length l = treeSize t}
 let rec preorder #x #b t = match t with
   | Leaf a -> [a]
-  | Branch a t1 t2 -> a :: (preorder t1) @ preorder t2
+  | Branch a t1 t2 -> begin
+    lemma_append_length (preorder t1) (preorder t2);
+    a :: (preorder t1) @ preorder t2
+  end
 
-(* Should I do a Lemma stating what preorder does? It'd look very similar to the implementation. *)
-
-val append_len: l1:list 'a -> l2:list 'a
-                -> Lemma (requires True)
-                        (ensures (length ( l1 @ l2) = length l1 + length l2))
-let rec append_len l1 l2 = match l1 with
-    | [] -> ()
-    | hd::tl -> append_len tl l2
-
-
-val random_lemma : 
-                 #b:Type -> 
-                 x:b -> 
-                 l1:list b -> 
-                 l2:list b -> 
-                 Lemma (length (x :: l1 @ l2) = 1 + length l1 + length l2)
-let rec random_lemma #b x l1 l2 = append_len (x::l1) l2
-
-val preorder_keeps_the_elements : #n:pos -> #b:Type -> t:comBiTree b n -> Lemma (length (preorder t) = treeSize t)
-let rec preorder_keeps_the_elements #n #b t = match t with
-    | Leaf _ -> ()
-    | Branch x t1 t2 -> begin
-      preorder_keeps_the_elements t1;
-      preorder_keeps_the_elements t2;
-      random_lemma x (preorder t1) (preorder t2)
-    end
-
-val preorder_has_the_root_first : 
-                                #n:pos -> 
-                                #b:eqtype ->
-                                x:b ->
-                                t1:comBiTree b n -> 
-                                t2:comBiTree b n -> 
-                                Lemma 
-                                  (preorder (Branch x t1 t2) = 
-                                    x :: ((preorder t1) @ (preorder t2)))
-let preorder_has_the_root_first #n #b x t1 t2 = () 
+//val lemma_preorder_has_the_root_first : 
+//                                #n:pos -> 
+//                                #b:eqtype ->
+//                                x:b ->
+//                                t1:comBiTree b n -> 
+//                                t2:comBiTree b n -> 
+//                                Lemma 
+//                                  (preorder (Branch x t1 t2) = 
+//                                    x :: ((preorder t1) @ (preorder t2)))
+//let lemma_preorder_has_the_root_first #n #b x t1 t2 = () 
 
 (* raNode
    It's a non empty linked list of strictly increasing comBiTrees
@@ -93,10 +117,10 @@ type raNode 'a : (n:pos) -> Type =
     | More : #m:pos -> #k:pos{k>m} -> comBiTree 'a m -> 
         raNode 'a k -> raNode 'a m
 
-val lenRan : #x:pos -> #b:Type -> r:raNode b x -> Tot (y:pos) (decreases r)
-let rec lenRan #x #b r  = match r with
+val ranLen : #x:pos -> #b:Type -> r:raNode b x -> Tot (y:pos) (decreases r)
+let rec ranLen #x #b r  = match r with
     | Last _ -> 1
-    | More _ m -> 1 + lenRan m
+    | More _ m -> 1 + ranLen m
 
 val toList : #x:pos -> #b:Type -> r:raNode b x -> Tot (list b) (decreases r)
 let rec toList #x #b r = match r with
@@ -105,10 +129,9 @@ let rec toList #x #b r = match r with
 
 val sizeRan : #x:pos -> #b:Type -> r:raNode b x -> Tot (y:pos{y = length (toList r)}) (decreases r)
 let rec sizeRan #x #b r = match r with
-    | Last t -> (preorder_keeps_the_elements t; treeSize t)
+    | Last t -> treeSize t
     | More t m -> begin
-      preorder_keeps_the_elements t;
-      append_len (preorder t) (toList m);
+      lemma_append_length (preorder t) (toList m);
       treeSize t + sizeRan m
     end
 
@@ -170,7 +193,19 @@ let raToList #b ra = match ra with
     | Once ran -> toList ran
     | Twice t r -> preorder t @ toList r
 
-val insert : #b:Type -> b -> ralist b -> ralist b
+val sizeRAList : #b:Type -> ralist b -> nat
+let sizeRAList #b rl = match rl with
+  | Empty -> 0
+  | Once rn -> sizeRan rn
+  | Twice t rn -> treeSize t + sizeRan rn
+
+val size_lemma : #b:Type -> rl:ralist b -> Lemma (sizeRAList rl = length (raToList rl))
+let size_lemma #b rl = match rl with
+  | Empty -> ()
+  | Once _ -> ()
+  | Twice t rn -> lemma_append_length (preorder t) (toList rn)
+
+val insert : #b:Type -> b -> rl:ralist b -> rl2:ralist b
 let insert #b a ral = match ral with
     | Empty -> Once (Last (Leaf a))
     | Once ran -> let sRan = treeHeight (headTree ran) in
@@ -187,19 +222,13 @@ let insert #b a ral = match ral with
                  else Twice newTree ran3
       end
 
-val helper_lemma : #b:eqtype -> x:b -> l1:list b -> l2:list b -> Lemma ((x::l1) @ l2 = x::(l1@l2))
-let rec helper_lemma #b x l1 l2 = ()
-
-val other_helper_lemma : #b:eqtype -> l1:list b -> l2:list b -> l3:list b -> Lemma ((l1@l2)@l3 = l1@(l2@l3))
-let rec other_helper_lemma #b l1 l2 l3 = match l1 with
-  | [] -> ()
-  | hd::tl -> (helper_lemma hd tl l2; helper_lemma hd (tl@l2) l3; other_helper_lemma tl l2 l3)
 
 val helper_fun : #b:Type -> ralist b -> bool
 let helper_fun #b r = match r with
-  | Empty -> true 
+  | Twice (Leaf _)  _ -> true 
   | _ -> false
-  
+
+// This states that insert behaves like :: on the list
 val insert_lemma : 
                  #b:eqtype -> 
                  x:b -> 
@@ -214,57 +243,31 @@ let insert_lemma #b x rl = match rl with
   end
   | Twice t ran2 -> begin
     match ran2 with 
-      | Last t2 -> preorder_has_the_root_first x t t2
-      | More t2 ran -> let newTree = Branch x t t2 in
-        if (treeHeight (headTree ran)) > (treeHeight newTree)
-        then (
-          preorder_has_the_root_first x t t2;
-          helper_lemma x (preorder t @ preorder t2) (toList ran);
-          other_helper_lemma (preorder t) (preorder t2) (toList ran)
-        )
-        else (
-          preorder_has_the_root_first x t t2; 
-          helper_lemma x (preorder t @ preorder t2) (toList ran);
-          other_helper_lemma (preorder t) (preorder t2) (toList ran)
-        )
+      | Last t2 -> ()
+      | More t2 ran -> lemma_append_assoc (preorder t) (preorder t2) (toList ran) 
   end
 
+// insert modifies the size as expected
+val insert_lemma_size : #b:Type -> x:b -> rl:ralist b -> Lemma (sizeRAList (insert x rl) = sizeRAList rl + 1)
+let insert_lemma_size #b x rl = begin 
+  size_lemma (insert x rl)
+end
 
-val lenNode : #b:Type -> #n:nat{n > 0} -> rs:raNode b n -> Tot (x:nat{x >= pow2 n - 1}) (decreases rs)
-let rec lenNode #b #n ran = match ran with
-  | Last t -> pow2 (treeHeight t) - 1
-  | More t ran2 -> pow2 (treeHeight t) - 1 + lenNode ran2
-
-val len : #b:Type -> ralist b -> Tot (x:nat)
-let len #b ral = match ral with
-  | Empty -> 0
-  | Once ran -> lenNode ran
-  | Twice t ran -> pow2 (treeHeight t) - 1 + lenNode ran
-
-
-val head : #b:Type -> l:ralist b{len l > 0} -> b
+val head : #b:Type -> l:ralist b{sizeRAList l > 0} -> b
 let head #b ral = match ral with
-  | Once ran -> begin match ran with
-      | Last t -> begin  match t with
-           | Leaf a -> a
-           | Branch a _ _ -> a
-           end
-      | More t _ -> begin match t with
-           | Leaf a -> a
-           | Branch a _ _ -> a
-           end
-      end
-  | Twice t _ -> begin match t with
-      | Leaf a -> a
-      | Branch a _ _ -> a
-      end
+  | Once ran -> treeRoot (headTree ran)
+  | Twice t _ -> treeRoot t
 
-val head_lemma : #b:eqtype -> x:b -> rl:ralist b{len rl > 0} -> Lemma (head (insert x rl) = x)
-let head_lemma #b x rl = insert_lemma x rl
+// head after an insert returns the inserted element
+val head_lemma : #b:eqtype -> x:b -> rl:ralist b -> Lemma (head (insert x rl) = x)
+let head_lemma #b x rl = ()
 
-
-val tail : #b:Type -> #n:pos -> l:ralist b{len l = n} -> m:ralist b{len m = n - 1}
-let tail #b #n ral = match ral with
+// head behaves as hd on the list version
+val head_lemma_2 : #b:eqtype -> rl:ralist b{sizeRAList rl > 0} -> Lemma (head rl = hd (raToList rl))
+let head_lemma_2 #b rl = ()
+  
+val ratail : #b:Type -> #n:pos -> l:ralist b{sizeRAList l = n} -> m:ralist b{sizeRAList m = n - 1}
+let ratail #b #n ral = match ral with
   | Once ran -> begin match ran with
          | Last t -> begin match t with
                 | Leaf _ -> Empty
@@ -280,8 +283,81 @@ let tail #b #n ral = match ral with
       | Branch _ t1 t2 -> Twice t1 (More t2 nxtRan)
     end
 
-//val tail_lemma : #b:Type -> x:b -> rl:ralist b -> Lemma (tail (insert x rl) = rl)
-//let
+// tailing after inserting gives back the same list
+val ratail_lemma : #b:eqtype -> #n:nat -> x:b -> rl:ralist b{sizeRAList rl = n} -> Lemma (ensures ratail #b #(n+1) (insert x rl) = rl)
+let rec ratail_lemma #b #n x rl = match rl with
+  | Empty -> ()
+  | Once ran -> begin 
+    match treeHeight (headTree ran) with
+      | 1 -> ()
+      | _ -> ()
+  end
+  | Twice t ran2 -> begin
+    match ran2 with 
+      | Last t2 -> ()
+      | More t2 ran -> 
+          lemma_append_assoc (preorder t) (preorder t2) (toList ran)
+  end
+
+// tail behaves as tail on the corresponding list
+val ratail_lemma_list : #b:eqtype -> #n:pos -> rl:ralist b{sizeRAList rl = n} -> Lemma (raToList (ratail #b #n rl) = tail (raToList rl))
+let ratail_lemma_list  #b #n rl = match rl with
+   | Once ran -> begin match ran with
+         | Last t -> begin match t with
+                | Leaf _ -> () //Empty
+                | Branch _ t1 t2 -> () //Twice t1 (Last t2)
+           end
+         | More t nxtRan -> begin match t with
+                | Leaf _ -> () //Once nxtRan
+                | Branch _ t1 t2 -> lemma_append_assoc (preorder t1) (preorder t2) (toList nxtRan) //Twice t1 (More t2 nxtRan)
+           end
+    end
+  | Twice t nxtRan -> begin match t with
+      | Leaf a -> () //Once nxtRan
+      | Branch _ t1 t2 -> lemma_append_assoc (preorder t1) (preorder t2) (toList nxtRan) //Twice t1 (More t2 nxtRan)
+    end
+
+// This says that deconstructing a list with tail and head, and then reconstructing it using the insert
+// gives the same list.
+// I think this gives a very strong result, saying that every ralist is equal to a list constructed with inserts, this
+// if stated correctly, could allow us to do a case on RAlists similar to list, ie, you can see a RAlist as a head and a tail, or 
+// an empty list
+val insert_inverse_head_tail : #b:eqtype -> #n:pos -> rl:ralist b{sizeRAList rl = n} -> Lemma (insert (head rl) (ratail #b #n rl) = rl)
+let insert_inverse_head_tail #b #n rl = match rl with
+  | Once ran -> begin match ran with
+         | Last t -> begin match t with
+                | Leaf _ -> () //Empty
+                | Branch _ t1 t2 -> () //Twice t1 (Last t2)
+           end
+         | More t nxtRan -> begin match t with
+                | Leaf _ -> () //Once nxtRan
+                | Branch _ t1 t2 -> lemma_append_assoc (preorder t1) (preorder t2) (toList nxtRan) //Twice t1 (More t2 nxtRan)
+           end
+    end
+  | Twice t nxtRan -> begin match t with
+      | Leaf a -> () //Once nxtRan
+      | Branch _ t1 t2 -> lemma_append_assoc (preorder t1) (preorder t2) (toList nxtRan) //Twice t1 (More t2 nxtRan)
+    end| Once ran -> ()
+  | Twice t ran -> ()
+
+
+
+val fromList : #b:eqtype -> l:list b -> rl:ralist b{raToList rl = l}
+let rec fromList #b l = match l with
+  | [] -> Empty
+  | hd::tl -> begin
+    insert_lemma hd (fromList tl);
+    insert hd (fromList tl)
+  end
+
+val fromList_toList_inverses : #b:eqtype -> rl:ralist b -> Lemma (rl = fromList (raToList rl))
+// fromList l = insert (hd l) (fromlist (tail l))
+// fromlist (toList rl) = insert (hd (toList rl)) (fromList (tail (toList rl)))
+// fromlist (toList rl) = insert (head rl) (fromlist (tolist (ratail rl)))
+let fromList_toList_inverses #b rl = match rl with
+  | Empty -> ()
+  | a -> begin match (head a, ratail a) with 
+    | (x, xs) -> 
 
 // fuel < 3*log2(i)
 val lookupTree : #b:Type -> #m:pos -> i:nat{i < pow2 m - 1}  -> #fuel:pos{fuel = m}(*Here I'd like to state that fuel == log2(i), it's stronger*) -> comBiTree b m -> b
@@ -326,3 +402,48 @@ let testList :ralist int  = insert 1 (insert 2 (insert 0 empty))
 *)
         
         
+
+//// Some results on the structure
+
+val tree_spine_eq : #b:Type -> #h1:pos -> #h2:pos -> t1:comBiTree b h1 -> t2:comBiTree b h2 -> r:bool{r = (h1 = h2)}
+let rec tree_spine_eq #b #h1 #h2 t1 t2 = match t1 with
+  | Leaf _ -> begin match t2 with
+    | Leaf _ -> true
+    | _ -> false
+  end
+  | Branch _ t11 t12 -> begin match t2 with
+    | Branch _ t21 t22 -> (tree_spine_eq t11 t21) &&  (tree_spine_eq t12 t22)
+    | _ -> false
+  end
+  | _ -> false
+
+val tree_spine_doesnt_depend_on_elements : #b:Type -> #h1:pos -> #h2:pos -> t1:comBiTree b h1 -> t2:comBiTree b h2 -> Lemma (requires treeSize t1 = treeSize t2) (ensures tree_spine_eq t1 t2)
+let tree_spine_doesnt_depend_on_elements #b #h1 #h2 t1 t2 = tree_size_gives_height t1 t2
+
+val node_spine_eq : #b:Type -> #s1:pos -> #s2:pos -> ran1:raNode b s1 -> ran2:raNode b s2 -> Tot (r:bool{r ==> (sizeRan ran1 = sizeRan ran2)}) (decreases ran1)
+let rec node_spine_eq #b #s1 #s2 ran1 ran2 = match ran1 with
+  | Last t1 -> begin match ran2 with
+    | Last t2 -> tree_spine_eq t1 t2
+    | _ -> false
+  end
+  | More t1 rran1 -> begin match ran2 with
+    | More t2 rran2 -> (tree_spine_eq t1 t2) && (node_spine_eq rran1 rran2)
+    | _ -> false
+  end
+
+//val node_spine_only_depends_on_size : #b:Type -> #s1:pos -> #s2:pos -> ran1:raNode b s1 -> ran2:raNode b s2 -> Lemma ((sizeRan ran1 = sizeRan ran2) ==> node_spine_eq ran1 ran2)
+
+
+val raspine_eq : #b:Type -> rl1:ralist b -> rl2:ralist b -> bool
+let rec raspine_eq #b rl1 rl2 = match (rl1, rl2) with
+  | (Empty, Empty) -> true
+  | (Once ran1, Once ran2) -> node_spine_eq ran1 ran2
+  | (Twice t1 ran1, Twice t2 ran2) -> tree_spine_eq t1 t2 && node_spine_eq ran1 ran2
+  | _ -> false 
+
+
+// This would be a very important proof, it would allow us to think about the structure
+// of the ralist only by its size, which would make most proofs easier
+// TODO do this, as of now I dont have a good intuiton on how to proceed, but its very related
+// to the theory of skew binary numbers
+//val spine_doesnt_depend_on_elements : #b:Type -> #n:pos -> rl1:ralist b{sizeRAList rl1 = n} -> rl2:ralist b{sizeRAList rl2 = n} -> Lemma (raspine_eq rl1 rl2)
